src/ml/coqIO.ml
@@ -1,0 +1,27 @@
+type std = StdOut | StdErr
+
+type 'a io = unit -> 'a
+
+let io_bind (c : 'a io) (f : 'a -> 'b io) : 'b io =
+  fun y -> 
+    let x = c () in
+    f x y
+
+let io_ret (x : 'a) : 'a io = fun _ -> x
+
+let io_printChar (c : char) : unit io =
+  fun _ -> print_char c
+
+let io_printCharF (s : std) (c : char) : unit io =
+  fun _ -> 
+    match s with
+      | StdOut -> print_char c
+      | StdErr -> prerr_char c
+
+let io_read : char io =
+  fun _ ->
+    input_char stdin
+  
+let run_io c = c ()
+
+let make_io c = c
