src/ml/coqIO.mli
@@ -1,0 +1,18 @@
+type std = StdOut | StdErr
+
+type 'a io
+
+val io_bind : 'a io -> ('a -> 'b io) -> 'b io
+
+val io_ret : 'a -> 'a io
+
+val io_printChar : char -> unit io
+
+val io_printCharF : std -> char -> unit io
+
+val io_read : char io
+
+(** Since ocaml internalizes IO **)
+val run_io : 'a io -> 'a 
+
+val make_io : (unit -> 'a) -> 'a io
