src/coq/Optimize.v
@@ -4,27 +4,24 @@ Require Import ExtLib.Structures.Monads.
 Set Implicit Arguments.
 Set Strict Implicit.
 
-Module Optimize.
+Section parametric.
+  Variable exp : Type.
+  Variable m : Type -> Type.
 
-  Section parametric.
-    Variable exp : Type.
-    Variable m : Type -> Type.
+  Definition optimization : Type := exp -> m exp.
+  
+  Context {Monad_m : Monad m}.
 
-    Definition optimization : Type := exp -> m exp.
-    
-    Context {Monad_m : Monad m}.
+  Fixpoint optSeq (os : list optimization) : optimization :=
+    match os with
+      | nil => fun x => ret x
+      | o :: os => fun x => bind (o x) (optSeq os)
+    end.
+  
+  Fixpoint optRepeat (n : nat) (o : optimization) : optimization :=
+    match n with
+      | 0 => o
+      | S n => fun x => bind (o x) (optRepeat n o)
+    end.
+End parametric.
 
-    Fixpoint optSeq (os : list optimization) : optimization :=
-      match os with
-        | nil => fun x => ret x
-        | o :: os => fun x => bind (o x) (optSeq os)
-      end.
-    
-    Fixpoint optRepeat (n : nat) (o : optimization) : optimization :=
-      match n with
-        | 0 => o
-        | S n => fun x => bind (o x) (optRepeat n o)
-      end.
-  End parametric.
-
-End Optimize.
