test/IONat.v
@@ -2,4 +2,4 @@ Require Import CoqIO.IO.
 Require Import ExtLib.Programming.Show.
 
 Definition main : IO unit :=
-  runShow (show 1).
+  runShow (M := ShowScheme_IO StdOut) (show 1).
